refactor spinlock

examples/include/spinlock.h
@@ -5,7 +5,6 @@
 #include <stdatomic.h>
 
 //@rc::require refinedc.examples.spinlock
-//@rc::import spinlock_annot from refinedc.examples.spinlock (for code only)
 //@rc::import spinlock_def from refinedc.examples.spinlock
 //@rc::context `{!lockG Σ}
 
@@ -22,13 +21,13 @@ void sl_init(struct spinlock* lock);
 
 [[rc::parameters("p : loc", "gamma : lock_id", "beta : own_state")]]
 [[rc::args("p @ &frac<beta, spinlock<gamma>>")]]
-[[rc::ensures("frac beta p : spinlock<gamma>", "[spinlock_token gamma []]")]]
+[[rc::ensures("frac beta p : spinlock<gamma>", "[lock_token gamma []]")]]
 void sl_lock(struct spinlock* lock);
 
 
 [[rc::parameters("p : loc", "gamma : lock_id", "beta : own_state")]]
 [[rc::args("p @ &frac<beta, spinlock<gamma>>")]]
-[[rc::requires("[spinlock_token gamma []]")]]
+[[rc::requires("[lock_token gamma []]")]]
 [[rc::ensures("frac beta p : spinlock<gamma>")]]
 [[rc::annot_args("0 : 1 LockA")]]
 void sl_unlock(struct spinlock* lock);
