linux/pkvm/proofs/spinlock/spinlock_def.v
@@ -1,11 +1,8 @@
-From refinedc.typing Require Import typing.
-From refinedc.linux.pkvm.spinlock Require Import spinlock_annot.
-From refinedc.linux.pkvm.spinlock Require Import generated_code.
 From iris.algebra Require Import csum excl auth cmra_big_op.
 From iris.algebra Require Import big_op gset gmap frac agree excl_auth.
+From refinedc.typing Require Import typing.
+From refinedc.linux.pkvm.spinlock Require Import generated_code.
 Set Default Proof Using "Type".
-
-Open Scope Z.
 
 Notation range k n := (seqZ k (n - k)) (only parsing).
 
@@ -21,22 +18,18 @@ Record lock_id := mk_lock_id {
 }.
 
 (** Registering the necessary ghost state. *)
-Class lockG Σ := LockG {
-   lock_inG :> inG Σ (authR (gset_disjUR string));
-   lock_excl_inG :> inG Σ (exclR unitO);
+Class spinlockG Σ := SpinLockG {
    lock_tickets_inG :> inG Σ (gmapR Z (exclR unitO));
    lock_owner_inG :> inG Σ (excl_authR ZO);
 }.
-Definition lockΣ : gFunctors :=
-  #[GFunctor (constRF (authR (gset_disjUR string)));
-    GFunctor (constRF (exclR unitO));
-    GFunctor (constRF (gmapR Z (exclR unitO)));
+Definition spinlockΣ : gFunctors :=
+  #[GFunctor (constRF (gmapR Z (exclR unitO)));
     GFunctor (constRF (excl_authR ZO))].
-Instance subG_lockG {Σ} : subG lockΣ Σ → lockG Σ.
+Instance subG_spinlockG {Σ} : subG spinlockΣ Σ → spinlockG Σ.
 Proof. solve_inG. Qed.
 
 Section type.
-  Context `{!typeG Σ} `{!lockG Σ}.
+  Context `{!typeG Σ} `{!lockG Σ} `{!spinlockG Σ}.
 
   Definition owner_auth (γ : gname) (i : Z) : iProp Σ :=
     own γ (●E i).
@@ -44,22 +37,8 @@ Section type.
   Definition owner_frag (γ : gname) (i : Z) : iProp Σ :=
     own γ (◯E i).
 
-  Definition lock_token_token (γ : gname) (l : list string) : iProp Σ :=
-    ∃ s : gset string, ⌜l ≡ₚ elements s⌝ ∗ own γ (● GSet s).
-
-  Definition lock_token (id : lock_id) (l : list string) : iProp Σ :=
-    ∃ i, lock_token_token id.(γ_lock) l ∗ owner_auth id.(γ_owner) i.
-
-  Theorem lock_token_token_exclusive (γ : gname) (l1 l2 : list string):
-    lock_token_token γ l1 -∗ lock_token_token γ l2 -∗ False.
-  Proof.
-    iIntros "H1 H2".
-    iDestruct "H1" as (?) "[? H1]".
-    iDestruct "H2" as (?) "[? H2]".
-    iCombine "H1 H2" as "H".
-    iDestruct (own_valid with "H") as %H%auth_auth_op_valid.
-    by iPureIntro.
-  Qed.
+  Definition spinlock_token (id : lock_id) (l : list string) : iProp Σ :=
+    ∃ i, lock_token id.(γ_lock) l ∗ owner_auth id.(γ_owner) i.
 
   Definition ticket_aux (γ : gname) (i : Z) : iProp Σ :=
     own γ {[i := Excl ()]} ∗ ⌜i ≠ NO_TICKET⌝.
@@ -141,13 +120,6 @@ Section type.
     by iApply (ticket_non_duplicable with "Ht1 Ht2").
   Qed.
 
-  Theorem alloc_lock_token_aux :
-    ⊢ |==> ∃ γ, lock_token_token γ [].
-  Proof.
-    iMod (own_alloc (● GSet ∅)) as (γ) "Hγ"; first by apply auth_auth_valid.
-    iModIntro. iExists γ, ∅. by iFrame.
-  Qed.
-
   Theorem alloc_tickets_aux_generic (ks : list Z) :
     Forall (λ i, i ≠ NO_TICKET) ks →
     NoDup ks →
@@ -199,11 +171,11 @@ Section type.
   Qed.
 
   Theorem alloc_lock_token_and_tickets :
-    ⊢ |==> ∃ id, lock_token id [] ∗
+    ⊢ |==> ∃ id, spinlock_token id [] ∗
                   ticket_range id 0 (LAST_TICKET + 1) ∗
                   owner_frag id.(γ_owner) 0.
   Proof.
-    iMod (alloc_lock_token_aux) as (γl) "Hγl".
+    iMod (alloc_lock_token) as (γl) "Hγl".
     iMod (alloc_tickets_aux) as (γt) "Hγt".
     iMod (alloc_auth_owner 0) as (γo) "[H● H◯]".
     iModIntro. iExists {|γ_lock := γl; γ_tickets := γt; γ_owner := γo|}.
@@ -228,7 +200,7 @@ Section type.
       owner_frag id.(γ_owner) owner ∗
       ticket_range id 0 owner ∗
       ticket_range id next (LAST_TICKET + 1) ∗
-      ((ticket id owner ∧ ⌜owner < next⌝) ∨ lock_token id [])
+      ((ticket id owner ∧ ⌜owner < next⌝) ∨ spinlock_token id [])
   )%I.
 
   Global Instance hyp_spinlock_t_timeless id o n: Timeless (hyp_spinlock_t_invariant id o n).
@@ -241,160 +213,7 @@ Section type.
       ) lockN (hyp_spinlock_t_invariant id p1 p2)
     )).
 
-  Program Definition spinlocked_ex {A} (id : lock_id) (n : string) (x : A) (ty : A → type) : type := {|
-    ty_own β l :=
-      match β return _ with
-      | Own => l ◁ₗ ty x
-      | Shr => ∃ γ', inv lockN ((∃ x', l ◁ₗ ty x' ∗ own γ' (Excl ())) ∨ own id.(γ_lock) (◯ GSet {[ n ]}))
-      end
-  |}%I.
-  Next Obligation.
-    iIntros (A γ n x ty l E HE) "Hl".
-    iMod (own_alloc (Excl ())) as (γ') "Hown" => //.
-    iExists _. iApply inv_alloc. iIntros "!#". iLeft. iExists _. by iFrame.
-  Qed.
-
-  Global Program Instance movable_spinlocked_ex A γ n x (ty : A → type) `{!Movable (ty x)}: Movable (spinlocked_ex γ n x ty) := {|
-    ty_layout := (ty x).(ty_layout);
-    ty_own_val v := (v ◁ᵥ (ty x))%I;
-  |}.
-  Next Obligation. iIntros (A γ n x ty ? v) "Hl". by iApply ty_aligned. Qed.
-  Next Obligation. iIntros (A γ n x ty ? v) "Hl". by iApply ty_size_eq. Qed.
-  Next Obligation. iIntros (A γ n x ty ? l) "Hl". by iApply ty_deref. Qed.
-  Next Obligation. iIntros (A γ n x ty ? l l') "Hl". by iApply ty_ref. Qed.
-
-  Lemma hyp_spinlock_t_subsume id1 id2 l T β:
-    ⌜id1 = id2⌝ ∗ T -∗
-    subsume (l ◁ₗ{β} hyp_spinlock_t id1) (l ◁ₗ{β} hyp_spinlock_t id2) T.
-  Proof. iIntros "[-> $] $". Qed.
-  Global Instance spinlock_subsume_inst id1 id2 l β:
-    Subsume (l ◁ₗ{β} hyp_spinlock_t id1) (l ◁ₗ{β} hyp_spinlock_t id2) :=
-    λ T, i2p (hyp_spinlock_t_subsume id1 id2 l T β).
-
-  Lemma spinlocked_simplify_hyp_place A γ n x (ty : A → type) T l:
-    (l ◁ₗ ty x -∗ T)  -∗
-    simplify_hyp (l ◁ₗ spinlocked_ex γ n x ty) T.
-  Proof. done. Qed.
-  Global Instance spinlocked_simplify_hyp_place_inst A γ n x (ty : A → type) l:
-    SimplifyHypPlace l Own (spinlocked_ex γ n x ty) (Some 0%N) :=
-    λ T, i2p (spinlocked_simplify_hyp_place A γ n x ty T l).
-
-  Lemma spinlocked_simplify_goal_place A γ n x (ty : A → type) T l:
-    T (l ◁ₗ ty x) -∗
-    simplify_goal (l ◁ₗ spinlocked_ex γ n x ty) T.
-  Proof. iIntros "HT". iExists _. iFrame. iIntros "$". Qed.
-
-  Global Instance spinlocked_simplify_goal_place_inst A γ n x (ty : A → type) l:
-    SimplifyGoalPlace l Own (spinlocked_ex γ n x ty) (Some 0%N) :=
-    λ T, i2p (spinlocked_simplify_goal_place A γ n x ty T l).
-
-  Lemma spinlocked_subsume A γ n x1 x2 (ty : A → type) l β T:
-    ⌜β = Own → x1 = x2⌝ ∗ T -∗
-    subsume (l ◁ₗ{β} spinlocked_ex γ n x1 ty) (l ◁ₗ{β} spinlocked_ex γ n x2 ty) T.
-  Proof. iIntros "[% $] Hl". by destruct β; naive_solver. Qed.
-  Global Instance spinlocked_subsume_inst A γ n x1 x2 (ty : A → type) l β:
-    Subsume (l ◁ₗ{β} spinlocked_ex γ n x1 ty) (l ◁ₗ{β} spinlocked_ex γ n x2 ty) | 10 :=
-    λ T, i2p (spinlocked_subsume A γ n x1 x2 ty l β T).
-
-  Definition spinlocked_ex_token {A} (id : lock_id) (n : string) (l : loc) (β : own_state) (ty : A → type)  : iProp Σ :=
-    (∀ E x, ⌜↑lockN ⊆ E⌝ -∗ l ◁ₗ ty x ={E}=∗ l ◁ₗ{β} spinlocked_ex id n x ty ∗ own id.(γ_lock) (◯ GSet {[ n ]}))%I.
-
-  Lemma locked_open A n s l id (x : A) ty β E:
-    n ∉ s → ↑lockN ⊆ E →
-    l ◁ₗ{β} spinlocked_ex id n x ty -∗
-      lock_token id s ={E}=∗
-      ▷ ∃ x', l ◁ₗ ty x' ∗ lock_token id (n :: s) ∗ spinlocked_ex_token id n l β ty ∗ ⌜β = Own → x = x'⌝.
-  Proof.
-    iIntros (Hnotin ?) "Hl Hlock". iDestruct "Hlock" as (?) "[Hlock H●]".
-    iDestruct "Hlock" as (st Hperm) "Hown". rewrite ->Hperm in Hnotin.
-    iMod (own_update with "Hown") as "[Hown Hs]". { eapply auth_update_alloc.
-      apply (gset_disj_alloc_empty_local_update st {[n]}). set_solver. }
-    rewrite {1}/ty_own /=.
-    iAssert (lock_token id (n :: s)) with "[Hown H●]" as "$". {
-      iExists _. iFrame. iExists _. iFrame. iPureIntro.
-      rewrite Hperm elements_union_singleton //. set_solver.
-    }
-    destruct β. { iIntros "!# !#". iExists _. iFrame. iSplit => //. eauto. }
-    iDestruct "Hl" as (γ') "#Hinv".
-    iInv "Hinv" as "[Hl|>Hn]" "Hc". 2: {
-      iDestruct (own_valid_2 with "Hs Hn") as %Hown. exfalso. move: Hown.
-      rewrite -auth_frag_op auth_frag_valid gset_disj_valid_op. set_solver.
-    }
-    iMod ("Hc" with "[Hs]") as "_". by iRight.
-    iIntros "!# !#". iDestruct "Hl" as (x') "[Hl Hexcl]".
-    iExists _. iFrame. iSplitL => //.
-    (** locked_token *)
-    iIntros (E' x'' ?) "Hl".
-    iInv "Hinv" as "[H|>$]" "Hc". 1: {
-      have ? : Inhabited A by apply (populate x).
-      iDestruct "H" as (?) "[_ >He]".
-        by iDestruct (own_valid_2 with "Hexcl He") as %Hown%exclusive_l.
-    }
-    iMod ("Hc" with "[Hl Hexcl]") as "_". 2: by iExists _.
-    iModIntro. iLeft. iExists _. iFrame.
-  Qed.
-
-  Lemma locked_close A n s l id (x : A) ty β E:
-    ↑lockN ⊆ E →
-    spinlocked_ex_token id n l β ty -∗ l ◁ₗ ty x -∗ lock_token id (n :: s) ={E}=∗
-    lock_token id s ∗ l ◁ₗ{β} spinlocked_ex id n x ty.
-  Proof.
-    iIntros (HE) "Hlocked Hl Hlock".
-    iMod ("Hlocked" with "[//] Hl") as "[$ Hn]".
-    iDestruct "Hlock" as (?) "[Hlock ?]".
-    iDestruct "Hlock" as (st Hst) "Htok".
-    iExists _. iFrame.
-    iExists (st ∖ {[n]}). iSplitR. {
-      iPureIntro. move: (Hst). rewrite {1}(union_difference_L {[n]} st).
-      rewrite ->elements_union_singleton => ?; last set_solver.
-      by apply: Permutation.Permutation_cons_inv.
-      set_unfold => ??. subst. apply elem_of_elements. rewrite -Hst. set_solver.
-    }
-    iCombine "Htok" "Hn" as "Htok".
-    iMod (own_update with "Htok") as "$" => //.
-    eapply auth_update_dealloc.
-      by apply gset_disj_dealloc_local_update.
-  Qed.
-
-  Lemma annot_unlock A l T β id n ty (x : A):
-    (find_in_context (FindDirect (lock_token id)) (λ s : list string, ⌜n∉s⌝ ∗ (∀ x',
-        lock_token id (n :: s) -∗ spinlocked_ex_token id n l β ty -∗ ⌜β = Own → x = x'⌝ -∗
-                       l ◁ₗ ty x' -∗ T))) -∗
-    typed_annot_stmt UnlockA l β (spinlocked_ex id n x ty) T.
-  Proof.
-    iDestruct 1 as (s) "(Hs&%&HT)". iIntros "Hlocked".
-    iMod (locked_open with "Hlocked Hs") as "Htok" => //.
-    iApply step_fupd_intro => //. iModIntro.
-    iDestruct "Htok" as (x') "(Hl&Hs&Htok&%)".
-    by iApply ("HT" with "Hs Htok [//] Hl").
-  Qed.
-  Global Instance annot_unlock_inst A l β γ n ty (x : A):
-    TypedAnnotStmt UnlockA l β (spinlocked_ex γ n x ty) :=
-    λ T, i2p (annot_unlock A l T β γ n ty x).
-
-  Lemma type_annot_lock (l : loc) (ty : mtype) T:
-    (∃ β id, subsume (l ◁ᵥ ty) (l ◁ₗ{β} hyp_spinlock_t id) (
-      find_in_context (FindDirect (lock_token id)) (λ s : list string, foldr (λ t T,
-        find_in_context (FindDirect (λ '(existT A (l2, ty)), spinlocked_ex_token (A:=A) id t l2 β ty)) (λ '(existT A (l2, ty)), ∃ x,
-          l2 ◁ₗ ty x ∗ (l2 ◁ₗ{β} spinlocked_ex id t x ty -∗ T))) (l ◁ₗ{β} hyp_spinlock_t id -∗ lock_token id [] -∗ T) s))) -∗
-    typed_annot_expr 1%nat LockA l ty T.
-  Proof.
-    iDestruct 1 as (β γ) "Hsub". iIntros "Hl".
-    iDestruct ("Hsub" with "Hl") as "[Hlock H]".
-    iDestruct "H" as (s) "[Htok Hs]".
-    iApply step_fupd_intro => //. iModIntro.
-    iInduction s as [|t s] "IH" => /=. by iApply ("Hs" with "Hlock Htok").
-    iDestruct "Hs" as ([A [l2 ty2]]) "[Hlt H]".
-    iDestruct "H" as (x) "[Hl HT]".
-    iMod (locked_close with "Hlt Hl Htok") as "[Htok Hl]" => //.
-    iApply ("IH" with "Hlock Htok"). by iApply "HT".
-  Qed.
-  Global Instance type_annot_lock_inst (l : loc) ty :
-    TypedAnnotExpr 1%nat LockA l ty :=
-    λ T, i2p (type_annot_lock l ty T).
+  Global Instance with_lock_id_hyp_spinlock_t id : WithLockId (hyp_spinlock_t id) (id.(γ_lock)) := I.
 End type.
 
-(* TODO> DO something stronger, e.g. sealing? *)
-Typeclasses Opaque hyp_spinlock_t spinlocked_ex lock_token spinlocked_ex_token.
-Notation spinlocked γ n ty := (spinlocked_ex γ n tt (λ _, ty)).
-Notation spinlocked_token γ n l β ty := (spinlocked_ex_token γ n l β (λ _ : unit, ty)).
+Typeclasses Opaque hyp_spinlock_t lock_token.
