examples/proofs/paper_example_2_1/generated_spec.v
@@ -80,11 +80,11 @@ Section spec.
   (* Specifications for function [sl_lock]. *)
   Definition type_of_sl_lock :=
     fn(∀ (p, gamma, beta) : loc * lock_id * own_state; (p @ (&frac{beta} (spinlock (gamma)))); True)
-      → ∃ () : (), (void); (p ◁ₗ{beta} (spinlock (gamma))) ∗ (spinlock_token gamma []).
+      → ∃ () : (), (void); (p ◁ₗ{beta} (spinlock (gamma))) ∗ (lock_token gamma []).
 
   (* Specifications for function [sl_unlock]. *)
   Definition type_of_sl_unlock :=
-    fn(∀ (p, gamma, beta) : loc * lock_id * own_state; (p @ (&frac{beta} (spinlock (gamma)))); (spinlock_token gamma []))
+    fn(∀ (p, gamma, beta) : loc * lock_id * own_state; (p @ (&frac{beta} (spinlock (gamma)))); (lock_token gamma []))
       → ∃ () : (), (void); (p ◁ₗ{beta} (spinlock (gamma))).
 
   (* Specifications for function [alloc]. *)
