linux/pkvm/proofs/early_alloc/instances.v
@@ -4,6 +4,9 @@ Set Default Proof Using "Type".
 Section instances.
   Context  `{!typeG Σ}.
 
+  Global Instance simpl_to_NULL_val_of_loc (l : loc) : SimplAndRel (=) NULL (l) (λ T, False).
+  Proof. split; naive_solver. Qed.
+
   Lemma simplify_goal_place_shift_loc_0nat_times l n β ty T:
     T (l ◁ₗ{β} ty) -∗ simplify_goal ((l +ₗ 0%nat * n) ◁ₗ{β} ty) T.
   Proof. iIntros "HT". assert (0%nat * n = 0) as -> by lia. rewrite shift_loc_0. iExists _. eauto with iFrame. Qed.
@@ -18,10 +21,17 @@ Section instances.
     SimplifyGoalPlace (l.1, l.2) β ty (Some 0%N) :=
     λ T, i2p (simplify_goal_place_combine l β ty T).
 
+  Lemma simplify_hyp_place_combine_offset l β n ty T:
+    ((l +ₗ n) ◁ₗ{β} ty -∗ T) -∗ simplify_hyp ((l.1, l.2 + n) ◁ₗ{β} ty) T.
+  Proof. iIntros "HT". iApply "HT". Qed.
+  Global Instance simplify_hyp_place_combine_offset_inst l β n ty:
+    SimplifyHypPlace (l.1, l.2 + n) β ty (Some 0%N) :=
+    λ T, i2p (simplify_hyp_place_combine_offset l β n ty T).
+
   Lemma simplify_goal_place_combine_offset l β n ty T:
     T ((l +ₗ n) ◁ₗ{β} ty) -∗ simplify_goal ((l.1, l.2 + n) ◁ₗ{β} ty) T.
   Proof. iIntros "HT". iExists _. eauto with iFrame. Qed.
   Global Instance simplify_goal_place_combine_offset_inst l β n ty:
-    SimplifyGoalPlace (l.1, l.2 + n) β ty (Some 0%N) | 100 :=
+    SimplifyGoalPlace (l.1, l.2 + n) β ty (Some 0%N) :=
     λ T, i2p (simplify_goal_place_combine_offset l β n ty T).
 End instances.
