linux/pkvm/proofs/spinlock/spinlock_annot.v
@@ -1,1 +1,0 @@
-Inductive LockAnnot : Type := LockA | UnlockA.
